update evm

src/program.v
@@ -5,6 +5,8 @@
 From mathcomp Require Import all_ssreflect.
 Require Import bitsops bitsrep instr.
 
+Require Import List.
+Import ListNotations.
 Require Import listhelp.
 
 (*=Program *)
@@ -18,15 +20,28 @@ Definition BYTEToOpCode (b : BYTE) : Instr :=
 
 
 (* Get BYTE at postion [pc], counting from 0 *)
-Definition getCodeAt (pc : nat) (pro : Program) : option BYTE :=
+Definition getCodeAt (pc : EVMWORD) (pro : Program) : option BYTE :=
+  let n := toNat pc in 
   if (nth_ok n pro (#0 : BYTE)) then
     Some (nth n pro (#0 : BYTE))
   else
     None.
            
-  
-(* Unit test *)
-Compute (BYTEToOpCode (#243 : BYTE)).
+
+(*---------------------------------------------------------------------
+ Unit test.
+ ---------------------------------------------------------------------*)
+Example pro1 : Program := [(#96:BYTE); (#0:BYTE); (#53:BYTE); (#84:BYTE); (#25:BYTE); (#96:BYTE); (#9:BYTE); (#87:BYTE); (#0:BYTE); (#91:BYTE); (#96:BYTE); (#32:BYTE); (#53:BYTE);
+                (#96:BYTE); (#0:BYTE); (#53:BYTE); (#85:BYTE)].
+
+Compute (
+    let oInstr := getCodeAt (#2:EVMWORD) pro1 in
+    match oInstr with
+      | Some b => BYTEToOpCode b
+      | None => BADINSTR
+    end
+  ).
+
 
 
 
