src/evm.v
@@ -1,12 +1,12 @@
-(*=============================================
+(*=================================================================================
  The Ethereum Virtual Machine
- =============================================*)
+ =================================================================================*)
 
 
 Require Import mathcomp.ssreflect.ssreflect.
 From mathcomp Require Import ssrfun ssrbool eqtype ssrnat seq fintype finfun tuple zmodp.
 
-Require Import bitsrep bitsops cursor pmap reader writer mem stack storage instr program state ere.
+Require Import bitsrep bitsops cursor pmap reader writer mem stack storage instr program ere.
 
 Set Implicit Arguments.
 Unset Strict Implicit.
@@ -20,12 +20,51 @@ Inductive EVMException :=
 | OutOfGas
 | OutOfStack
 | StackUnderflow.
+(*=End *)
 
 (*=EVM *)
 Record EVMachine :=
   mkEVMachine {
+      (* EVM state *)
+      g : EVMWORD;
+      pc : EVMWORD;
+      m :> Mem;
+      i : EVMWORD;
+      s :> Stack;
+      (* external environment *)
       m_ere : EREnvironment;
-      m_evmstate : EVMState;
       m_storage : Storage
     }.
+(*=End *)
 
+
+(*----------------------------------------------------------------------------
+ Stop.
+ ----------------------------------------------------------------------------*)
+Definition eval_STOP (s1 : EVMachine) : (option EVMException) * EVMachine :=
+  (None, s1).
+
+(*---------------------------------------------------------------------------
+ Arithmetic operations.
+ ---------------------------------------------------------------------------*)
+Definition eval_ADD (s1 : EVMachine) : (option EVMException) * EVMachine :=
+  let current_ere := s1.(m_ere) in
+  let current_stack := s1.(s) in
+  let ores := @add2top current_stack in
+  match ores with
+    | None => (Some StackUnderflow, s1)
+    | Some next_stack => (None, mkEVMachine s1.(g) (incB s1.(pc)) s1.(m) s1.(i) next_stack s1.(m_ere) s1.(m_storage))
+  end.
+
+
+
+
+(*-----------------------------------------------------------------------------
+ Operational Semantics of the EVM.
+ The evaluation of the bytecode included in [m_ere] takes the [initState] and 
+ results the final state or exception.
+ If there exits any exception, the final state is the initialized state.
+ -----------------------------------------------------------------------------*)
+(*Fixpoint EVMEvaluation (initState : EVMachine) : (option EVMException) * EVMachine :=
+*)
+  
